Stateful SHA2: functional correctness of the block counter in the initialization function

code/experimental/hash/Hacl.Hash.SHA2.L256.fst
@@ -347,22 +347,35 @@ val alloc:
 let alloc () = Buffer.create (u32_to_h32 0ul) size_state
 
 
+#reset-options "--max_fuel 0  --z3rlimit 10"
+
 val init:
   state:uint32_p{length state = v size_state} ->
   Stack unit
-    (requires (fun h0 -> live h0 state))
+    (requires (fun h0 -> live h0 state
+              /\ (let seq_counter = Seq.slice (as_seq h0 state) (U32.v pos_count_w) (U32.(v pos_count_w + v size_count_w)) in
+              let counter = Seq.index seq_counter 0 in
+              H32.v counter = 0)))
     (ensures  (fun h0 r h1 -> live h1 state /\ modifies_1 state h0 h1
               /\ (let slice_k = Seq.slice (as_seq h1 state) (U32.v pos_k_w) (U32.(v pos_k_w + v size_k_w)) in
               let slice_h_0 = Seq.slice (as_seq h1 state) (U32.v pos_whash_w) (U32.(v pos_whash_w + v size_whash_w)) in
+              let seq_counter = Seq.slice (as_seq h1 state) (U32.v pos_count_w) (U32.(v pos_count_w + v size_count_w)) in
+              let counter = Seq.index seq_counter 0 in
               let seq_k = Hacl.Spec.Endianness.reveal_h32s slice_k in
               let seq_h_0 = Hacl.Spec.Endianness.reveal_h32s slice_h_0 in
-              seq_k == Spec.k /\ seq_h_0 == Spec.h_0)))
+              seq_k == Spec.k /\ seq_h_0 == Spec.h_0 /\ H32.v counter = 0)))
+
+#reset-options "--max_fuel 0  --z3rlimit 50"
 
 let init state =
+  (**) let h0 = ST.get () in
+  let n = Buffer.sub state pos_count_w size_count_w in
   let k = Buffer.sub state pos_k_w size_k_w in
   let h_0 = Buffer.sub state pos_whash_w size_whash_w in
   constants_set_k k;
-  constants_set_h_0 h_0
+  constants_set_h_0 h_0;
+  (**) let h1 = ST.get () in
+  (**) no_upd_lemma_2 h0 h1 k h_0 n
 
 
 [@"substitute"]
